Verify semantics of read_all and some renaming in rel.v

lib/rel.v
@@ -12,15 +12,134 @@ From ExtLib Require Import
      Data.Monads.OptionMonad
      Structures.Monads.
 
-From SimpleIO Require Import
-     IOMonad CoqPervasives Utils.
-
 From advent.lib Require Import
      io.
 
 (* State [s -> (s * a)] as a relation. *)
 Definition state_rel (S : Type) (A : Type) : Type :=
   S -> S -> A -> Prop.
+
+Instance Monad_state_rel (S : Type) : Monad (state_rel S) := {
+  ret _ x := fun s1 s2 x' => s2 = s1 /\ x' = x;
+  bind _ _ m k := fun s1 s3 y =>
+    exists x s2, m s1 s2 x /\ k x s2 s3 y
+}.
+
+Instance MonadError_state_rel (S : Type) : MonadError (state_rel S) := {
+  error _ _ := fun _ _ _ => False
+}.
+
+Definition incl_rel {S A : Type} (r1 r2 : state_rel S A) :=
+  forall s1 s2 a, r1 s1 s2 a -> r2 s1 s2 a.
+
+Definition eq_rel {S A : Type} (r1 r2 : state_rel S A) :=
+  incl_rel r1 r2 /\ incl_rel r2 r1.
+
+Definition incl_rel1 {S A B : Type}
+           (r1 r2 : A -> state_rel S B) :=
+  forall x, incl_rel (r1 x) (r2 x).
+
+Lemma incl_rel1_refl {S A B : Type} (r : A -> state_rel S B) :
+  incl_rel1 r r.
+Proof.
+  intros x z1 z2 y; auto.
+Qed.
+
+Inductive lfp_rel1 {S A B : Type}
+          (gf : (A -> state_rel S B) -> (A -> state_rel S B))
+          (a : A) (s1 s2 : S) (b : B) : Prop :=
+| LFP
+    (P : A -> state_rel S B)
+    (P_ind : incl_rel1 P (lfp_rel1 gf))
+    (P_holds : gf P a s1 s2 b).
+
+Definition monotonic_rel {S U V A : Type}
+           (gf : (U -> state_rel S V) -> state_rel S A) :=
+  forall r1 r2,
+    incl_rel1 r1 r2 ->
+    incl_rel (gf r1) (gf r2).
+
+Definition monotonic_rel1 {S U V A B : Type}
+           (gf : (U -> state_rel S V) -> (A -> state_rel S B)) :=
+  forall r1 r2,
+    incl_rel1 r1 r2 ->
+    incl_rel1 (gf r1) (gf r2).
+
+Lemma lfp_rel_unfold {S A B : Type}
+      (gf : (A -> state_rel S B) -> (A -> state_rel S B))
+      (mon_gf : monotonic_rel1 gf) :
+  incl_rel1 (lfp_rel1 gf) (gf (lfp_rel1 gf)).
+Proof.
+  intros x z1 z2 y [P P_ind P_holds].
+  eapply mon_gf.
+  apply P_ind.
+  apply P_holds.
+Qed.
+
+Lemma lfp_rel_fold {S A B : Type}
+      (gf : (A -> state_rel S B) -> (A -> state_rel S B)) :
+  incl_rel1 (gf (lfp_rel1 gf)) (lfp_rel1 gf).
+Proof.
+  intros x z1 z2 y Hgf.
+  apply LFP with (P := lfp_rel1 gf).
+  apply incl_rel1_refl.
+  auto.
+Qed.
+
+Lemma really_lfp {S A B : Type}
+      (gf : (A -> state_rel S B) -> (A -> state_rel S B))
+      (mon_gf : monotonic_rel1 gf)
+      (fp : A -> state_rel S B)
+      (H_fp : incl_rel1 (gf fp) fp) :
+  incl_rel1 (lfp_rel1 gf) fp.
+Proof.
+  intros x z1 z2 y.
+  induction 1 as [x z1 z2 y P P_ind IH P_holds].
+  apply H_fp.
+  apply mon_gf with (r1 := P); auto.
+Qed.
+
+Instance MonadFix_state_rel (S : Type) : MonadFix (state_rel S) := {
+  mfix _ _ := lfp_rel1
+}.
+
+(* Utilities to prove monotonicity. *)
+
+Lemma monotonic_refl (S U V W A : Type)
+      (m : state_rel S A) :
+  monotonic_rel1 (fun (_ : U -> _ V) (_ : W) => m).
+Proof.
+  unfold monotonic_rel1, incl_rel1, incl_rel; auto.
+Qed.
+
+Lemma monotonic_id (S U V W : Type)
+      (g : W -> U) :
+  monotonic_rel1 (fun (f : U -> state_rel S V) (w : W) => f (g w)).
+Proof.
+  unfold monotonic_rel1, incl_rel1; auto.
+Qed.
+
+Lemma monotonic_ret (S U V W A : Type)
+      (g : W -> A) :
+  monotonic_rel1 (fun (f : U -> state_rel S V) (w : W) => ret (g w)).
+Proof.
+  unfold monotonic_rel1, incl_rel1, incl_rel; auto.
+Qed.
+
+Lemma monotonic_bind (S U V W A B : Type)
+      (m : (U -> state_rel S V) -> W -> state_rel S A)
+      (k : (U -> state_rel S V) -> W -> A -> state_rel S B)
+      (mon_m : monotonic_rel1 m)
+      (mon_k : forall a, monotonic_rel1 (fun f w => k f w a)) :
+  monotonic_rel1 (fun f w => pbind (m f w) (k f w)).
+Proof.
+  intros r1 r2 Hr12 w s1 s3 b [a [s2 [Hm Hk]]].
+  exists a, s2.
+  firstorder.
+  specialize (mon_k a).
+  unfold monotonic_rel1 in mon_k.
+  eapply mon_k; eauto.
+Qed.
 
 Record io_state (I O : Type) := Mk_io_state {
   input : list I;
@@ -53,23 +172,13 @@ Definition rel_spec (I O : Type) :
       x (initial i) s tt /\
       output s = o.
 
-Instance Monad_state_rel (S : Type) : Monad (state_rel S) := {
-  ret _ x := fun s1 s2 x' => s2 = s1 /\ x' = x;
-  bind _ _ m k := fun s1 s3 y =>
-    exists x s2, m s1 s2 x /\ k x s2 s3 y
-}.
-
-Instance MonadError_state_rel (S : Type) : MonadError (state_rel S) := {
-  error _ _ := fun _ _ _ => False
-}.
-
 Instance MonadI_io_rel (I O : Type) : MonadI I (io_rel I O) := {
   read := fun s1 s2 x' =>
     (exists z,
       input s1 = z :: input s2 /\
       s2 = drop_input s1 /\
       x' = Some z) \/
-    (s2 = s1 /\ x' = None);
+    (input s1 = [] /\ s2 = s1 /\ x' = None);
 }.
 
 Instance MonadO_io_rel (I O : Type) : MonadO O (io_rel I O) := {
@@ -78,67 +187,85 @@ Instance MonadO_io_rel (I O : Type) : MonadO O (io_rel I O) := {
     x' = tt
 }.
 
-Definition incl_rel {S A : Type} (r1 r2 : state_rel S A) :=
-  forall s1 s2 a, r1 s1 s2 a -> r2 s1 s2 a.
-
-Definition incl_rel_1 {S A B : Type}
-           (r1 r2 : A -> state_rel S B) :=
-  forall x, incl_rel (r1 x) (r2 x).
-
-Lemma incl_rel_1_refl {S A B : Type} (r : A -> state_rel S B) :
-  incl_rel_1 r r.
+Lemma read_all_rel {I O : Type} :
+  eq_rel read_all
+         (fun (s1 s2 : io_state I O) xs =>
+            xs = input s1 /\
+            s2 = Mk_io_state [] (output s1)).
 Proof.
-  intros x z1 z2 y; auto.
+  split.
+  - intros s1 s2 xs.
+    unfold read_all.
+    match goal with
+    | [ |- mfix ?body _ _ _ _ -> _ ] =>
+      assert (mon_body : monotonic_rel1 body)
+    end.
+    { apply monotonic_bind.
+      - apply monotonic_refl.
+      - intros [i|].
+        { apply monotonic_id. }
+        { apply monotonic_ret. }
+    }
+    match goal with
+    | [ |- mfix ?body _ _ _ _ -> _ ] =>
+      assert (H : forall acc s1 s2 xs,
+                 lfp_rel1 body acc s1 s2 xs ->
+                 xs = rev acc ++ input s1 /\
+                 s2 = Mk_io_state [] (output s1))
+    end.
+    { revert mon_body; clear; intros mon_body acc [is1 os1].
+      revert acc. induction is1 as [| i1 is1]; intros acc s2 xs Hloop.
+      - apply lfp_rel_unfold in Hloop; auto.
+        destruct Hloop as [ox [s1' [Hread Hloop]]].
+        destruct Hread as [[i1 [Hi1]] | [Hi [Hs1' Hox]]].
+        + discriminate Hi1.
+        + subst ox.
+          destruct Hloop; subst; simpl.
+          split.
+          * rewrite app_nil_r. rewrite rev_alt. reflexivity.
+          * reflexivity.
+      - apply lfp_rel_unfold in Hloop; auto.
+        destruct Hloop as [ox [s1' [Hread Hloop]]].
+        destruct Hread as [[i1' [Hi1 [Hs1' Hox]]] | [Hs1' Hox]].
+        + subst ox s1'.
+          simpl in Hi1; inversion Hi1; subst.
+          apply IHis1 in Hloop.
+          destruct Hloop as [Hxs Hs2]. subst.
+          simpl.
+          rewrite <- app_assoc.
+          auto.
+        + discriminate.
+    }
+    apply H.
+  - intros s1 s2 is1 [His1 Hs2].
+    unfold read_all.
+    match goal with
+    | [ |- mfix ?body _ _ _ _ ] =>
+      assert (H : forall acc s1 s2 is1,
+                 is1 = rev acc ++ input s1 ->
+                 s2 = Mk_io_state [] (output s1) ->
+                 lfp_rel1 body acc s1 s2 is1)
+    end.
+    { clear.
+      intros acc s1. revert acc.
+      remember (input s1) as is1 eqn:Hs1.
+      generalize dependent s1.
+      induction is1 as [|i1 is1 IH];
+        intros s1 Hs1 acc s2 xs His1 Hs2;
+        apply lfp_rel_fold.
+      + exists None, s2.
+        rewrite app_nil_r in His1.
+        split.
+        * right; destruct s1, s2; simpl in *; subst; auto.
+        * rewrite rev_alt in His1; simpl; auto.
+      + exists (Some i1), (Mk_io_state is1 (output s1)).
+        split.
+        * left. exists i1. simpl.
+          destruct s1; simpl in *; subst; auto.
+        * apply IH; auto.
+          simpl.
+          rewrite <- app_assoc.
+          auto.
+    }
+    apply H; auto.
 Qed.
-
-Inductive lfp_rel {S A B : Type}
-          (gf : (A -> state_rel S B) -> (A -> state_rel S B))
-          (a : A) (s1 s2 : S) (b : B) : Prop :=
-| LFP
-    (P : A -> state_rel S B)
-    (P_ind : incl_rel_1 P (lfp_rel gf))
-    (P_holds : gf P a s1 s2 b).
-
-Definition monotonic_rel {S A B : Type}
-           (gf : (A -> state_rel S B) -> (A -> state_rel S B)) :=
-  forall r1 r2,
-    incl_rel_1 r1 r2 ->
-    incl_rel_1 (gf r1) (gf r2).
-
-Lemma lfp_rel_unfold {S A B : Type}
-      (gf : (A -> state_rel S B) -> (A -> state_rel S B))
-      (mon_gf : monotonic_rel gf) :
-  incl_rel_1 (lfp_rel gf) (gf (lfp_rel gf)).
-Proof.
-  intros x z1 z2 y [P P_ind P_holds].
-  eapply mon_gf.
-  apply P_ind.
-  apply P_holds.
-Qed.
-
-Lemma lfp_rel_fold {S A B : Type}
-      (gf : (A -> state_rel S B) -> (A -> state_rel S B)) :
-  incl_rel_1 (gf (lfp_rel gf)) (lfp_rel gf).
-Proof.
-  intros x z1 z2 y Hgf.
-  apply LFP with (P := lfp_rel gf).
-  apply incl_rel_1_refl.
-  auto.
-Qed.
-
-Lemma really_lfp {S A B : Type}
-      (gf : (A -> state_rel S B) -> (A -> state_rel S B))
-      (mon_gf : monotonic_rel gf)
-      (fp : A -> state_rel S B)
-      (H_fp : incl_rel_1 (gf fp) fp) :
-  incl_rel_1 (lfp_rel gf) fp.
-Proof.
-  intros x z1 z2 y.
-  induction 1 as [x z1 z2 y P P_ind IH P_holds].
-  apply H_fp.
-  apply mon_gf with (r1 := P); auto.
-Qed.
-
-Instance MonadFix_state_rel (S : Type) : MonadFix (state_rel S) := {
-  mfix _ _ := lfp_rel
-}.
